Path.v
@@ -53,7 +53,7 @@ Module PathTheories  (O: UsualOrderedType)(S: FSetInterface.Sfun O)(G: Graph O S
     - eapply path_trans. apply p_start. apply H. apply IHpath'.
 Qed.
 
-  Fixpoint path_list (g: graph) (u v : vertex) (l: list vertex) : bool :=
+ (* Fixpoint path_list (g: graph) (u v : vertex) (l: list vertex) : bool :=
     match l with
     | nil => contains_edge g u v
     | w :: t => contains_edge g u w && path_list g w v t
@@ -73,7 +73,7 @@ Qed.
       + simpl in H. apply p_start'. apply H.
       + simpl in H. rewrite andb_true_iff in H. destruct H.  eapply p_continue'.  apply H.
         apply IHx. apply H0.
-  Qed.
+  Qed.*)
 
   Inductive path_with: graph -> vertex -> vertex -> (vertex -> bool) -> Prop :=
     |  pw_start : forall g u v f,
@@ -85,6 +85,37 @@ Qed.
       f v = true ->
       contains_edge g w v = true ->
       path_with g u v f.
+
+  Inductive path_list_ind: graph -> vertex -> vertex -> (vertex -> bool) -> list vertex -> Prop :=
+    | pl_start : forall g u v f,
+      contains_edge g u v = true ->
+      f v = true ->
+      path_list_ind g u v f nil
+    | pl_continue: forall g u v w f l,
+      path_list_ind g u w f l ->
+      f v = true ->
+      contains_edge g w v = true ->
+      path_list_ind g u v f (w :: l).
+
+Fixpoint path_list_rev (g: graph) (u v: vertex) (l: list vertex) : bool :=
+  match l with
+  | nil => G.contains_edge g u v
+  | x :: tl => G.contains_edge g x v && path_list_rev g u x tl
+  end.
+
+Lemma path_list_ind_rev: forall g u v l f,
+  path_list_ind g u v f l <-> (path_list_rev g u v l = true /\ (forall y, In y l -> f y = true) /\ f v = true).
+Proof.
+  intros. split; intros. induction H.
+  - simpl in *. split. apply H. split. intros. destruct H1. apply H0.
+  - simpl. destruct IHpath_list_ind. destruct H3. split. rewrite H1. rewrite H2. reflexivity.
+    split. intros. destruct H5. subst. apply H4. apply H3. apply H5. apply H0.
+  - generalize dependent v. induction l; intros.
+    + destruct H. destruct H0. simpl in *. apply pl_start. apply H. apply H1.
+    + simpl in *. apply pl_continue. apply IHl. destruct H. destruct H0. split. rewrite andb_true_iff in H.
+      apply H. split. intros. apply H0. right. apply H2. apply H0. left. reflexivity. destruct H.
+      destruct H0. apply H1. destruct H. rewrite andb_true_iff in H. destruct H. apply H.
+Qed. 
 
   Lemma path_with_implies_path: forall g u v f,
     path_with g u v f ->
